Refinery/Term/Extrinsic/Subst.lean
@@ -29,8 +29,24 @@ def Deriv?.splitRight {Γ : Ctx? α ε} {u v w : Var? α ε} {a : Term φ (Ty α
   | .left _, D => D.erase | .sboth _, D => D
   | .right _, D => D
 
+def Deriv?.unused {Γ : Ctx? α ε} {v : Var? α ε} (hΓ : Γ.del)  (a : Term φ (Ty α)) (hv : v.unused)
+  : (Γ ⊢? a : v) := match v with | ⟨A, 0, e⟩ => .zero hΓ a A e
+
+theorem Deriv?.copy {Γ : Ctx? α ε} {v : Var? α ε} {a : Term φ (Ty α)}
+  (D : Γ ⊢? a : v) (hv : v.used) (hc : v.copy) : Γ.copy := by cases D with
+  | valid D q hΓ =>
+    cases q using EQuant.casesZero with
+    | zero => cases hv
+    | rest q =>
+      constructor
+      rw [<-EQuant.coe_le_coe]
+      apply le_trans _ hΓ
+      simp [Var?.copy_iff] at hc
+      exact hc.q
+  | zero => cases hv
+
 inductive SubstDS (φ) {α ε} [S : Signature φ α ε] : Ctx? α ε → Ctx? α ε → Type _
-  | nil {Γ} (hΓ : Γ.del) : SubstDS φ Γ nil
+  | nil {Γ} (hΓ : Γ.del) : SubstDS φ Γ .nil
   | cons {Γ Γl Γr Δ} {v} {a : Term φ _} (hΓ : Γ.PSSplit Γl Γr)
     (σ : SubstDS φ Γl Δ) (da : Γr ⊢? a : v) : SubstDS φ Γ (Δ.cons v)
 
@@ -65,6 +81,58 @@ def SubstDS.headD {Γ Δ} : (σ : SubstDS φ Γ Δ) → σ.headCtx ⊢? (σ.toSu
 def SubstDS.tail {Γ Δ} : (σ : SubstDS φ Γ Δ) → SubstDS φ σ.tailCtx Δ.tail
   | .nil hΓ => .nil hΓ
   | .cons _ σ _ => σ
+
+structure SubstSplit (φ) {α ε} [S : Signature φ α ε] (inCtx outCtx outLeft outRight : Ctx? α ε)
+  where
+  (inLeft inRight : Ctx? α ε)
+  (splitIn : inCtx.PSSplit inLeft inRight)
+  (substLeft : SubstDS φ inLeft outLeft)
+  (substRight : SubstDS φ inRight outRight)
+
+def SubstSplit.erase_right (Γ : Ctx? α ε) [hΓ : Γ.del] : SubstSplit φ Γ .nil .nil .nil
+  := ⟨Γ, Γ.erase, Γ.erase_right, .nil hΓ, .nil inferInstance⟩
+
+def SubstSplit.erase_left (Γ : Ctx? α ε) [hΓ : Γ.del] : SubstSplit φ Γ .nil .nil .nil
+  := ⟨Γ.erase, Γ, Γ.erase_left, .nil inferInstance, .nil hΓ⟩
+
+def SubstDS.split {Γ Δl Δr : Ctx? α ε}
+  : SubstDS φ Γ Δ → Δ.PSSplit Δl Δr → SubstSplit φ Γ Δ Δl Δr
+  | .nil hΓ, .nil => SubstSplit.erase_right _
+  | .cons (Γr := Γr) (v := v) (a := a) hΓ σ da, .cons hΔ hlr =>
+    let s := σ.split hΔ
+    match hlr with
+    | .left _ =>
+      let Ξ := hΓ.c12_3_23 s.splitIn.comm
+      let s1_23 : Γ.PSSplit s.inRight Ξ := hΓ.s12_3_1_23 s.splitIn.comm
+      let s23 : Ξ.PSSplit s.inLeft Γr := hΓ.s12_3_23 s.splitIn.comm
+      ⟨Ξ, s.inRight,
+        s1_23.comm,
+        s.substLeft.cons s23 da,
+        s.substRight.cons s.inRight.erase_right (.zero inferInstance a _ _)⟩
+    | .right _ =>
+      let Ξ := hΓ.c12_3_23 s.splitIn
+      let s1_23 : Γ.PSSplit s.inLeft Ξ := hΓ.s12_3_1_23 s.splitIn
+      let s23 : Ξ.PSSplit s.inRight Γr := hΓ.s12_3_23 s.splitIn
+      ⟨s.inLeft, Ξ,
+        s1_23,
+        s.substLeft.cons s.inLeft.erase_right (.zero inferInstance a _ _),
+        s.substRight.cons s23 da⟩
+    | .sboth h =>
+      if hv : v.used then
+        have sr := Γr.both (hΓ := da.copy hv h.copy);
+        ⟨hΓ.c12_34_13 s.splitIn sr, hΓ.c12_34_24 s.splitIn sr,
+          hΓ.s12_34_13_24 s.splitIn sr,
+          s.substLeft.cons (hΓ.s12_34_13 s.splitIn sr) da,
+          s.substRight.cons (hΓ.s12_34_24 s.splitIn sr) da⟩
+      else
+        have hv := ((Var?.unused_iff _).mpr hv);
+        let Ξ := hΓ.c12_3_23 s.splitIn
+        let s1_23 : Γ.PSSplit s.inLeft Ξ := hΓ.s12_3_1_23 s.splitIn
+        let s23 : Ξ.PSSplit s.inRight Γr := hΓ.s12_3_23 s.splitIn
+        ⟨s.inLeft, Ξ,
+          s1_23,
+          s.substLeft.cons s.inLeft.erase_right (.unused inferInstance a hv),
+          s.substRight.cons s23 da⟩
 
 -- def SubstDS.splitLeft {Γ Δ Δl Δr} : SubstDS φ Γ Δ → Δ.PSSplit Δl Δr → Ctx? α ε
 --   | _ => sorry
